[REVERT THIS] too slow... why?

examples/mult/MultHeader.v
@@ -17,14 +17,55 @@ Set Implicit Arguments.
 
 
 
-Instance multRA: URA.t := Excl.t Z%ra.
+Instance fRA: URA.t := Excl.t Z%ra.
+Instance gRA: URA.t := Excl.t bool%ra.
+Instance hRA: URA.t := Excl.t nat%ra.
+Definition fpre: fRA := Some 5%Z.
+Definition fpost: fRA := Some 7%Z.
+Definition gpre: gRA := Some true.
+Definition gpost: gRA := Some false.
+Definition hpre: hRA := Some 15.
+Definition hpost: hRA := Some 17.
 
 Section PROOF.
 
-  Context `{@GRA.inG multRA Σ}.
+  Context `{@GRA.inG fRA Σ}.
+  Context `{@GRA.inG gRA Σ}.
+  Context `{@GRA.inG hRA Σ}.
 
-  Definition f_spec: fspec := mk_simple (fun (_: unit) => ((fun varg o => (OwnM (Some 5%Z) ** ⌜o = ord_top⌝)%I),
-                                                           (fun vret => (OwnM (Some 7%Z))%I))).
-  Definition GlobalStb: gname -> option fspec := to_stb [("f", f_spec)].
+  Definition f_spec0: fspec := mk_simple (fun (_: unit) => ((fun varg o => (OwnM fpre ** ⌜o = ord_top⌝)%I),
+                                                           (fun vret => (OwnM fpost)%I))).
+  Definition f_spec1: fspec := mk_simple (fun (_: unit) => ((fun varg o => (OwnM fpre ** OwnM gpre ** ⌜o = ord_top⌝)%I),
+                                                           (fun vret => (OwnM fpost ** OwnM gpost)%I))).
+  Definition g_spec: fspec := mk_simple (fun (_: unit) => ((fun varg o => (OwnM gpre ** ⌜o = ord_top⌝)%I),
+                                                           (fun vret => (OwnM gpost)%I))).
+  Definition h_spec0: fspec := fspec_trivial.
+  Definition h_spec1: fspec := mk_simple (fun (_: unit) => ((fun varg o => (OwnM hpre ** ⌜o = ord_top⌝)%I),
+                                                           (fun vret => (OwnM hpost)%I))).
 
+  Definition GlobalStb0: list (gname * fspec).
+    eapply (Seal.sealing "stb").
+    apply [("f", f_spec0); ("g", g_spec); ("h", h_spec0)].
+  Defined.
+
+  Definition GlobalStb1: list (gname * fspec).
+    eapply (Seal.sealing "stb").
+    apply [("f", f_spec1); ("g", g_spec); ("h", h_spec1)].
+  Defined.
+
+  (* Definition GlobalStb0: gname -> option fspec := to_stb [("f", f_spec0); ("g", g_spec); ("h", h_spec0)]. *)
+  (* Definition GlobalStb1: gname -> option fspec := to_stb [("f", f_spec1); ("g", g_spec); ("h", h_spec1)]. *)
+
+  (***
+(f) arg/ret only
+(g) tgt call meaningful spec
+(h) tgt call trivial spec
+
+update
+module resource
+APC
+   ***)
 End PROOF.
+
+Global Hint Unfold GlobalStb0: stb.
+Global Hint Unfold GlobalStb1: stb.
