examples/mult/Mult1.v
@@ -15,11 +15,14 @@ Set Implicit Arguments.
 
 
 Section PROOF.
-  Context `{@GRA.inG multRA Σ}.
+  Context `{@GRA.inG fRA Σ}.
+  Context `{@GRA.inG gRA Σ}.
+  Context `{@GRA.inG hRA Σ}.
 
   Definition multSbtb: list (gname * fspecbody) :=
     (* [("fire", mk_specbody f_spec (fun _ => trigger (Choose _)))]. *)
-    [("fire", mk_specbody f_spec (fun _ => Ret Vundef↑))].
+    (* [("f", mk_specbody f_spec0 (fun _ => `_: val <- ccallU "g" tt;; `_: val <- ccallU "h" tt;; Ret Vundef↑))]. *)
+    [("f", mk_specbody f_spec0 (fun _ => Ret Vundef↑))].
 
   Definition SMultSem: SModSem.t := {|
     SModSem.fnsems := multSbtb;
